terrible copy/paste hack (i'm sorry) to get BetreeBlockCache spec'ed out

disk-betree/BetreeSpec.dfy
@@ -3,6 +3,7 @@ include "../lib/sequences.dfy"
 include "../lib/Maps.dfy"
 include "MapSpec.dfy"
 include "Graph.dfy"
+include "BlockCache.dfy"
 
 module BetreeGraph refines Graph {
   import MS = MapSpec
@@ -89,7 +90,7 @@ module BetreeSpec refines BetreeSpecCommon {
     && WFNode(oldroot)
     && var newroot := AddMessageToNode(oldroot, key, msg);
     && var writeop := G.WriteOp(Root(), newroot);
-    && Tr.Transaction(k, s, s', [writeop])
+    && Tr.OpTransaction(k, s, s', [writeop])
   }
 
   predicate Flush(k: Tr.Constants, s: Tr.Variables, s': Tr.Variables, parentref: Reference, parent: Node, childref: Reference, child: Node, newchildref: Reference) {
@@ -105,7 +106,7 @@ module BetreeSpec refines BetreeSpecCommon {
     && var newparent := Node(newparentchildren, newparentbuffer);
     && var allocop := G.AllocOp(newchildref, newchild);
     && var writeop := G.WriteOp(parentref, newparent);
-    && Tr.Transaction(k, s, s', [allocop, writeop])
+    && Tr.OpTransaction(k, s, s', [allocop, writeop])
   }
 
   predicate Grow(k: Tr.Constants, s: Tr.Variables, s': Tr.Variables, oldroot: Node, newchildref: Reference) {
@@ -116,7 +117,7 @@ module BetreeSpec refines BetreeSpecCommon {
         imap key | MS.InDomain(key) :: []);
     && var allocop := G.AllocOp(newchildref, newchild);
     && var writeop := G.WriteOp(Root(), newroot);
-    && Tr.Transaction(k, s, s', [allocop, writeop])
+    && Tr.OpTransaction(k, s, s', [allocop, writeop])
   }
 
   predicate ValidFusion(fusion: NodeFusion)
@@ -152,7 +153,7 @@ module BetreeSpec refines BetreeSpecCommon {
     && var allocop_left := G.AllocOp(fusion.left_childref, fusion.left_child);
     && var allocop_right := G.AllocOp(fusion.right_childref, fusion.right_child);
     && var writeop := G.WriteOp(fusion.parentref, fusion.split_parent);
-    && Tr.Transaction(k, s, s', [allocop_left, allocop_right, writeop])
+    && Tr.OpTransaction(k, s, s', [allocop_left, allocop_right, writeop])
   }
 
   predicate Merge(k: Tr.Constants, s: Tr.Variables, s': Tr.Variables, fusion: NodeFusion)
@@ -163,6 +164,96 @@ module BetreeSpec refines BetreeSpecCommon {
     && ValidFusion(fusion)
     && var allocop := G.AllocOp(fusion.fused_childref, fusion.fused_child);
     && var writeop := G.WriteOp(fusion.parentref, fusion.fused_parent);
-    && Tr.Transaction(k, s, s', [allocop, writeop])
+    && Tr.OpTransaction(k, s, s', [allocop, writeop])
+  }
+}
+
+module BetreeGraphBlockCache refines BlockCache {
+  import G = BetreeGraph
+}
+
+module BetreeSpecForBlockCache refines BetreeSpecCommon {
+  import Tr = BetreeGraphBlockCache
+
+  predicate InsertMessage(k: Tr.Constants, s: Tr.Variables, s': Tr.Variables, key: Key, msg: BufferEntry, oldroot: Node) {
+    && Tr.Reads(k, s, Root(), oldroot)
+    && WFNode(oldroot)
+    && var newroot := AddMessageToNode(oldroot, key, msg);
+    && var writeop := G.WriteOp(Root(), newroot);
+    && Tr.OpTransaction(k, s, s', [writeop])
+  }
+
+  predicate Flush(k: Tr.Constants, s: Tr.Variables, s': Tr.Variables, parentref: Reference, parent: Node, childref: Reference, child: Node, newchildref: Reference) {
+    var movedKeys := iset k | k in parent.children && parent.children[k] == childref;
+    && Tr.Reads(k, s, parentref, parent)
+    && Tr.Reads(k, s, childref, child)
+    && WFNode(parent)
+    && WFNode(child)
+    && var newbuffer := imap k :: (if k in movedKeys then parent.buffer[k] + child.buffer[k] else child.buffer[k]);
+    && var newchild := Node(child.children, newbuffer);
+    && var newparentbuffer := imap k :: (if k in movedKeys then [] else parent.buffer[k]);
+    && var newparentchildren := imap k | k in parent.children :: (if k in movedKeys then newchildref else parent.children[k]);
+    && var newparent := Node(newparentchildren, newparentbuffer);
+    && var allocop := G.AllocOp(newchildref, newchild);
+    && var writeop := G.WriteOp(parentref, newparent);
+    && Tr.OpTransaction(k, s, s', [allocop, writeop])
+  }
+
+  predicate Grow(k: Tr.Constants, s: Tr.Variables, s': Tr.Variables, oldroot: Node, newchildref: Reference) {
+    && Tr.Reads(k, s, Root(), oldroot)
+    && var newchild := oldroot;
+    && var newroot := Node(
+        imap key | MS.InDomain(key) :: newchildref,
+        imap key | MS.InDomain(key) :: []);
+    && var allocop := G.AllocOp(newchildref, newchild);
+    && var writeop := G.WriteOp(Root(), newroot);
+    && Tr.OpTransaction(k, s, s', [allocop, writeop])
+  }
+
+  predicate ValidFusion(fusion: NodeFusion)
+  {
+    && fusion.left_keys !! fusion.right_keys
+    && (forall key :: key in fusion.left_keys ==> IMapsTo(fusion.fused_parent.children, key, fusion.fused_childref))
+    && (forall key :: key in fusion.left_keys ==> IMapsTo(fusion.split_parent.children, key, fusion.left_childref))
+
+    && (forall key :: key in fusion.right_keys ==> IMapsTo(fusion.fused_parent.children, key, fusion.fused_childref))
+    && (forall key :: key in fusion.right_keys ==> IMapsTo(fusion.split_parent.children, key, fusion.right_childref))
+
+    && (forall key :: (key !in fusion.left_keys) && (key !in fusion.right_keys) ==>
+      IMapsAgreeOnKey(fusion.split_parent.children, fusion.fused_parent.children, key))
+
+    && fusion.fused_parent.buffer == fusion.split_parent.buffer
+
+    && (forall key :: key in fusion.left_keys ==> IMapsAgreeOnKey(fusion.fused_child.children, fusion.left_child.children, key))
+    && (forall key :: key in fusion.left_keys ==> IMapsAgreeOnKey(fusion.fused_child.buffer, fusion.left_child.buffer, key))
+
+    && (forall key :: key in fusion.right_keys ==> IMapsAgreeOnKey(fusion.fused_child.children, fusion.right_child.children, key))
+    && (forall key :: key in fusion.right_keys ==> IMapsAgreeOnKey(fusion.fused_child.buffer, fusion.right_child.buffer, key))
+  }
+
+  predicate Split(k: Tr.Constants, s: Tr.Variables, s': Tr.Variables, fusion: NodeFusion)
+  {
+    && Tr.Reads(k, s, fusion.parentref, fusion.fused_parent)
+    && Tr.Reads(k, s, fusion.fused_childref, fusion.fused_child)
+    && ValidFusion(fusion)
+    && WFNode(fusion.fused_parent)
+    && WFNode(fusion.fused_child)
+    && WFNode(fusion.left_child)
+    && WFNode(fusion.right_child)
+    && var allocop_left := G.AllocOp(fusion.left_childref, fusion.left_child);
+    && var allocop_right := G.AllocOp(fusion.right_childref, fusion.right_child);
+    && var writeop := G.WriteOp(fusion.parentref, fusion.split_parent);
+    && Tr.OpTransaction(k, s, s', [allocop_left, allocop_right, writeop])
+  }
+
+  predicate Merge(k: Tr.Constants, s: Tr.Variables, s': Tr.Variables, fusion: NodeFusion)
+  {
+    && Tr.Reads(k, s, fusion.parentref, fusion.split_parent)
+    && Tr.Reads(k, s, fusion.left_childref, fusion.left_child)
+    && Tr.Reads(k, s, fusion.right_childref, fusion.right_child)
+    && ValidFusion(fusion)
+    && var allocop := G.AllocOp(fusion.fused_childref, fusion.fused_child);
+    && var writeop := G.WriteOp(fusion.parentref, fusion.fused_parent);
+    && Tr.OpTransaction(k, s, s', [allocop, writeop])
   }
 }
